EffectSSA/Trace/Lemmas.lean
@@ -1,0 +1,31 @@
+import EffectSSA.Trace.Defs
+
+/-!
+# Trace lemmas
+-/
+namespace EffectSSA
+variable {τ : Ty} [MemorySignature τ]
+
+namespace Trace
+
+/-! ## Basic constructor lemmas -/
+section Basic
+variable (e : Event τ) (es ds : List (Event τ))
+
+@[simp] theorem cons_seq : e :> (seq es) = seq (e :: es) := rfl
+@[simp] theorem seq_append_seq : (seq es) ++ (seq ds) = seq (es ++ ds) := rfl
+
+end Basic
+
+
+/-! ## `events` lemmas -/
+theorem eq_of_mem_events {es : Trace τ} (h : z ∈ es.events) :
+    es = z.pre ++ (z.event :> z.post) := by
+  simp only [events, Fin.getElem_fin] at h
+  split at h
+  · contradiction
+  · rcases z
+    simp only [Set.mem_setOf_eq, TraceZipper.mk.injEq] at h
+    rcases h with ⟨i, h⟩
+    repeat (rcases h with ⟨rfl, h⟩)
+    simp
